Free.fst
@@ -1,0 +1,52 @@
+module Free
+
+open Common
+
+noeq
+type cmd_sig (op:Type u#a) = {
+  args:(op -> Type u#a);
+  res:(op -> Type u#a);
+}
+
+noeq
+type freef op (s : cmd_sig op) a =
+  | Call : (l:op) -> (s.args l) -> (maybe (s.res l) -> a) -> freef op s a
+
+val freef_fmap : (#a:Type) -> (#b:Type) -> (#op:Type) -> (#s:cmd_sig op) ->
+                m:freef op s a -> (x:a{x<<m} -> b) -> freef op s b
+let freef_fmap #a #b #op #s m f=
+  match m with
+  | Call cmd args fnc -> Call cmd args (fun i -> FStar.WellFounded.axiom1 fnc i; f (fnc i))
+
+noeq
+type free (op:Type u#o) (s:cmd_sig op) (a:Type u#a) : Type u#(max o a) =
+  | Cont : freef op s (free op s a) -> free op s a
+  | Return : a -> free op s a
+  // TODO: is this relevant? can be made a silent cmd
+  | Throw : exn -> free op s a
+
+let free_return (op:Type) (s:cmd_sig op) (a:Type) (x:a)   : free op s a = Return x
+let free_throw  (op:Type) (s:cmd_sig op) (a:Type) (x:exn) : free op s a = Throw x 
+
+let rec free_bind (op:Type u#o) (s:cmd_sig op) (a:Type u#a) (b:Type u#b) (l : free op s a) (k : a -> free op s b) : free op s b =
+  match l with
+  | Return x -> k x 
+  | Throw err -> Throw err 
+  | Cont t -> Cont (freef_fmap t (fun fnci ->
+      free_bind op s a b fnci k))
+
+val lift_error : (#op:Type) -> (#s:cmd_sig op) -> (#a:Type) -> (maybe a) -> free op s a
+let lift_error #op #s #a v =
+  match v with
+  | Inl x -> free_return op s a x
+  | Inr err -> free_throw op s a err
+
+val free_perform : (#op:Type) -> (#s:cmd_sig op) -> (#a:Type) -> freef op s (maybe a) -> free op s a
+let free_perform #op #s #a v = 
+  free_bind op s (maybe a) (a) 
+    (Cont (freef_fmap #(maybe a) #_ v Return))
+    lift_error
+
+let free_map (op:Type u#o) (s:cmd_sig op) (a:Type u#a) (b:Type u#b) (l : free op s a) (k : a -> b) : free op s b =
+  free_bind op s a b 
+    l (fun a -> free_return op s b (k a))
